Weidenbach_Book/WB_More_Refinement.thy
@@ -632,6 +632,35 @@ lemma fref_to_Down_unRET:
   unfolding fref_def uncurry_def nres_rel_def
   by auto
 
+lemma fref_to_Down_unRET_uncurry2:
+  fixes f :: \<open>'a \<Rightarrow> 'b \<Rightarrow> 'c \<Rightarrow> 'f\<close>
+    and g :: \<open>'a2 \<Rightarrow> 'b2 \<Rightarrow> 'c2 \<Rightarrow> 'g\<close>
+  shows
+    \<open>(uncurry2 (RETURN ooo f), uncurry2 (RETURN ooo g)) \<in> [P]\<^sub>f A \<rightarrow> \<langle>B\<rangle>nres_rel \<Longrightarrow>
+       (\<And>(x :: 'a) x' y y' (z :: 'c) (z' :: 'c2).
+         P ((x', y'), z') \<Longrightarrow> (((x, y), z), ((x', y'), z')) \<in> A \<Longrightarrow>
+         (f x y z, g x' y' z') \<in> B)\<close>
+  unfolding fref_def uncurry_def nres_rel_def
+  by auto
+
+lemma fref_to_Down_unRET_uncurry3:
+  shows
+    \<open>(uncurry3 (RETURN oooo f), uncurry3 (RETURN oooo g)) \<in> [P]\<^sub>f A \<rightarrow> \<langle>B\<rangle>nres_rel \<Longrightarrow>
+       (\<And>(x :: 'a) x' y y' (z :: 'c) (z' :: 'c2) a a'.
+         P (((x', y'), z'), a') \<Longrightarrow> ((((x, y), z), a), (((x', y'), z'), a')) \<in> A \<Longrightarrow>
+         (f x y z a, g x' y' z' a') \<in> B)\<close>
+  unfolding fref_def uncurry_def nres_rel_def
+  by auto
+
+lemma fref_to_Down_unRET_uncurry4:
+  shows
+    \<open>(uncurry4 (RETURN ooooo f), uncurry4 (RETURN ooooo g)) \<in> [P]\<^sub>f A \<rightarrow> \<langle>B\<rangle>nres_rel \<Longrightarrow>
+       (\<And>(x :: 'a) x' y y' (z :: 'c) (z' :: 'c2) a a' b b'.
+         P ((((x', y'), z'), a'), b') \<Longrightarrow> (((((x, y), z), a), b), ((((x', y'), z'), a'), b')) \<in> A \<Longrightarrow>
+         (f x y z a b, g x' y' z' a' b') \<in> B)\<close>
+  unfolding fref_def uncurry_def nres_rel_def
+  by auto
+  
 
 subsubsection \<open>More Simplification Theorems\<close>
 
